theories/SLFRich.v
@@ -602,8 +602,9 @@ Proof using.
     { xpull. intros x q L' ->. xseq. xapp. xapp. xapp. xapp.
       (* Here takes place the recursive call, with frame on the head cell: *)
       xapply (IH L'). { auto. } intros _. 
-      xchange <- MList_cons. xsimpl. { rew_list. math. }  }
-    { xpull. intros ->. xval. xsimpl. auto. subst. xchange* <- (MList_nil null). } }
+      xchange <- MList_cons. { auto. } { xsimpl. rew_list. math. }  }
+    { xpull. intros ->. xval. xsimpl. { congruence. } 
+      subst. xchange* <- (MList_nil null). } }
   xapply KR. xpull. xapp. xapp. xapp. xval. xsimpl. math.
 Qed.
 
