theories/SepBaseAltProofs.v
@@ -831,7 +831,7 @@ Lemma triple_alloc : forall n,
     (fun r => \exists l, \[r = val_loc l /\ l <> null] \* Alloc (abs n) l).
 Proof using. (* Note: [abs n] currently does not compute in Coq. *)
   introv N Hh.
-  forwards~ (l&Dl&Nl): (Fmap.conseq_fresh null h (abs n) val_uninitialized).
+  forwards~ (l&Dl&Nl): (Fmap.conseq_fresh null h (LibList.make (abs n) val_uninitialized)).
   match type of Dl with Fmap.disjoint ?hc _ => sets h1': hc end.
   exists (h1' \u h) (val_loc l). splits~.
   { applys (eval_alloc (abs n)); eauto.
